---
layout: post
author: yiyangshi
title: "Yiyang's Chapter 3 Exercise"
---

Here is Exercise 1:
<iframe src="https://trinket.io/embed/python/5dc5a59fd2" width="100%" height="600" frameborder="0" marginwidth="0" marginheight="0" allowfullscreen></iframe>

Here is Exercise 2:
<iframe src="https://trinket.io/embed/python/bcd1999d91" width="100%" height="600" frameborder="0" marginwidth="0" marginheight="0" allowfullscreen></iframe>

Here is Exercise 3:
<iframe src="https://trinket.io/embed/python/ab5360f1cc" width="100%" height="600" frameborder="0" marginwidth="0" marginheight="0" allowfullscreen></iframe>

Reflection:
I noticed that the "if-if-if-..." expression can serve the same purpose as the "if-elif-elif-..." expression. I wonder if one is better than the other. My guess is the "if-if-if" expression is better because once the "if" statement is determined as false, the computer goes to the next "if" without having to "memorize" anything. For the "if-elif-elif" case, the range of the "elif" is the whole range minus the "if" range. So the computer has to find out the range first and then determine if a statement is true or false. Not sure if my guess is correct.
